ZFuniv.v
@@ -1,0 +1,263 @@
+Require Import Sat.
+Require Import ZF ZFcoc ZFord ZFgrothendieck.
+Require Import ZFlambda.
+
+Set Implicit Arguments.
+
+(** * Auxiliary lemmas: *)
+
+Lemma G_CCLam U :
+  grot_univ U ->
+  omega ∈ U ->
+  CCLam ∈ U.
+intros.
+assert (U_singl := G_singl _ H).
+assert (U_N : ZFnats.N ∈ U).
+ apply G_N; trivial.
+assert (U_0 : ZFnats.zero ∈ U).
+ apply G_inf_nontriv; trivial.
+assert (U_succ : forall n, n ∈ U -> ZFnats.succ n ∈ U).
+ intros.
+ apply G_union2; auto.
+unfold CCLam.
+unfold Lam.Lambda.
+apply G_TI; trivial.
+ do 2 red; intros.
+ unfold Lam.LAMf.
+ rewrite H1; reflexivity.
+
+ intros.
+ unfold Lam.LAMf.
+ auto 20 using G_union2, G_prodcart.
+Qed.
+Hint Resolve G_CCLam.
+
+(** * Encoding of types *)
+
+Definition mkTY x S := couple x (iSAT S).
+Definition Elt T := fst T. (* total elements *)
+Definition El T := union2 (singl empty) (Elt T). (* partial elements *)
+Definition Real T := sSAT (snd T) .
+
+Instance El_morph : morph1 El.
+do 2 red; intros; apply union2_morph; auto with *.
+apply fst_morph; trivial.
+Qed.
+
+Lemma El_mkTY T A : El (mkTY T A) == singl empty ∪ T.
+unfold El, Elt, mkTY; rewrite fst_def; reflexivity.
+Qed.
+Lemma Real_mkTY T A : eqSAT (Real (mkTY T A)) A.
+unfold Real, mkTY; rewrite snd_def; apply iSAT_id.
+Qed.
+
+Lemma Elt_El x y : x ∈ Elt y -> x ∈ El y.
+intros; apply union2_intro2; trivial.
+Qed.
+Lemma empty_El y : empty ∈ El y.
+apply union2_intro1; apply singl_intro.
+Qed.
+Hint Resolve Elt_El empty_El.
+
+(** * Universes *)
+
+(** Given K a set of set of values, builds a type of types (a sort), such that:
+    - types are neutral term (hence the Real field of the sort is SN)
+    - for each set of values and each saturated, there is a type built from
+      this data.
+ *)
+Definition sn_sort K := mkTY (sup K (fun P => replSAT (fun A => mkTY P A))) snSAT.
+
+Lemma sort_repl_morph :
+  Proper (eq_set ==> eqSAT ==> eq_set) (fun P A => mkTY P A).
+do 3 red; intros.
+apply couple_morph; trivial.
+apply iSAT_morph; trivial.
+Qed.
+Lemma sort_repl_morph2 :
+  Proper (eq_set ==> eq_set) (fun P => replSAT(fun A => mkTY P A)).
+do 2 red; intros.
+apply ZFrepl.repl_morph_raw; auto with *.
+do 2 red; intros.
+rewrite H1.
+unfold mkTY; rewrite H.
+rewrite (iSAT_morph _ _ (sSAT_morph _ _ H0)).
+reflexivity.
+Qed.
+Hint Resolve sort_repl_morph sort_repl_morph2.
+
+Lemma sn_sort_intro K T A :
+  T ∈ K -> mkTY T A ∈ El (sn_sort K).
+intros.
+unfold sn_sort; rewrite El_mkTY; apply union2_intro2.
+rewrite sup_ax; auto.
+exists T; trivial.
+rewrite replSAT_ax; auto.
+2:apply sort_repl_morph; reflexivity.
+exists A; reflexivity.
+Qed.
+
+Lemma sn_sort_elim_raw K T :
+  T ∈ El (sn_sort K) -> T == empty \/ exists U A, T == mkTY U A /\ U ∈ K.
+unfold sn_sort; rewrite El_mkTY.
+intro.
+apply union2_elim in H; destruct H.
+ apply singl_elim in H; auto.
+
+ rewrite sup_ax in H; auto.
+ destruct H as (U,?,?).
+ rewrite replSAT_ax in H0.
+ 2:apply sort_repl_morph; reflexivity.
+ destruct H0 as (A,?).
+ eauto.
+Qed.
+
+Lemma sn_sort_elim K T : T ∈ El (sn_sort K) -> T == empty \/ Elt T ∈ K.
+intros.
+apply sn_sort_elim_raw in H; destruct H as [?|(U,(A,(?,?)))]; auto.
+right; rewrite H.
+unfold Elt, mkTY; rewrite fst_def; trivial.
+Qed.
+
+Lemma sort_incl K1 K2 :
+  K1 ⊆ K2 ->
+  El (sn_sort K1) ⊆ El (sn_sort K2).
+red; intros.
+apply sn_sort_elim_raw in H0; destruct H0 as [?|(U,(A,(?,?)))].
+ rewrite H0; auto.
+
+ rewrite H0; apply sn_sort_intro; auto.
+Qed.
+
+Lemma Real_sort_sn K : eqSAT (Real (sn_sort K)) snSAT.
+apply Real_mkTY.
+Qed.
+
+Lemma sn_sort_in_type K1 K2 :
+  grot_univ K2 ->
+  omega ∈ K2 ->
+  K1 ∈ K2 ->
+  sn_sort K1 ∈ El (sn_sort K2).
+intros.
+apply sn_sort_intro.
+apply G_sup; intros; auto.
+apply G_replf; auto.
+ do 2 red; intros; apply couple_morph; auto with *.
+ apply iSAT_morph; apply sSAT_morph; trivial.
+
+ apply G_power; auto.
+
+ intros.
+ apply G_couple; trivial.
+  apply G_trans with K1; trivial.
+
+ apply G_subset; auto.
+Qed.
+
+Lemma El_in_grot K T :
+  grot_univ K -> 
+  empty ∈ K ->
+  T ∈ El (sn_sort K) ->
+  El T ∈ K.
+intros K_grot K_ne T_in_K.
+assert (Kse : singl empty ∈ K).
+ auto using G_singl.
+apply sn_sort_elim in T_in_K; destruct T_in_K.
+ apply G_union2; trivial.
+ rewrite H.
+ apply G_union; trivial.
+ apply G_subset; trivial.
+ apply G_union; trivial.
+
+ apply G_union2; auto.
+Qed.
+
+Definition sn_props := sn_sort props.
+
+Lemma El_in_props P :
+  P ∈ El sn_props ->
+  El P ∈ props.
+intros.
+apply cc_dec_prop.
+apply sn_sort_elim in H; destruct H; trivial.
+rewrite H.
+apply power_intro; intros.
+apply union_elim in H0; destruct H0.
+apply subset_elim1 in H1.
+apply union_elim in H1; destruct H1.
+apply empty_ax in H2; contradiction.
+Qed.
+
+
+(** * Dependent product *)
+
+Definition piSAT A (F:set->SAT) :=
+  prodSAT (Real A) (interSAT (fun p:{y|y ∈ El A} => F (proj1_sig p))).
+
+Definition sn_prod A F :=
+  mkTY (cc_prod (El A) (fun x => El (F x)))
+       (piSAT A (fun x => Real (F x))).
+
+Definition sn_lam A F := cc_lam (El A) F.
+
+Lemma sn_prod_intro : forall dom f F,
+  ext_fun (El dom) f ->
+  ext_fun (El dom) F ->
+  (forall x, x ∈ El dom -> f x ∈ El (F x)) ->
+  sn_lam dom f ∈ El (sn_prod dom F).
+intros.
+unfold sn_lam, sn_prod; rewrite El_mkTY.
+apply union2_intro2.
+apply cc_prod_intro; intros; auto.
+do 2 red; intros.
+apply El_morph; auto.
+Qed.
+
+Lemma sn_prod_elim : forall dom f x F,
+  f ∈ El (sn_prod dom F) ->
+  x ∈ El dom ->
+  cc_app f x ∈ El (F x).
+intros.
+unfold sn_prod in H; rewrite El_mkTY in H.
+apply union2_elim in H; destruct H.
+ apply singl_elim in H.
+ rewrite H.
+ rewrite cc_app_empty; auto.
+
+ apply cc_prod_elim with (dom:=El dom) (F:=fun x => El(F x)); trivial.
+Qed.
+
+(** * Dependent product and universes *)
+
+Lemma sn_predicative_prod : forall K dom F,
+  grot_univ K ->
+  empty ∈ K ->
+  ext_fun (El dom) F ->
+  dom ∈ El (sn_sort K) ->
+  (forall x, x ∈ El dom -> F x ∈ El (sn_sort K)) ->
+  sn_prod dom F ∈ El (sn_sort K).
+intros K dom F K_grot K_ne ext_F dom_ty F_ty.
+apply sn_sort_intro.
+apply G_cc_prod; trivial.
+ do 2 red; intros.
+ apply union2_morph; auto with *.
+ apply fst_morph.
+ apply ext_F; auto.
+
+ apply El_in_grot; trivial.
+
+ intros.
+ specialize F_ty with (1:=H).
+ apply El_in_grot; trivial.
+Qed.
+
+Lemma sn_impredicative_prod : forall dom F,
+  ext_fun (El dom) F ->
+  (forall x, x ∈ El dom -> F x ∈ El sn_props) ->
+  sn_prod dom F ∈ El sn_props.
+intros.
+apply sn_sort_intro.
+apply cc_impredicative_prod; intros.
+specialize H0 with (1:=H1).
+apply El_in_props; trivial.
+Qed.
