ZFuniv_real.v
@@ -1,0 +1,445 @@
+Require Import Sat.
+Require Import ZF ZFcoc ZFord ZFgrothendieck.
+Require Import ZFlambda.
+
+Set Implicit Arguments.
+
+(** * Auxiliary lemmas: *)
+
+Lemma G_CCLam U :
+  grot_univ U ->
+  omega ∈ U ->
+  CCLam ∈ U.
+intros.
+assert (U_singl := G_singl _ H).
+assert (U_N : ZFnats.N ∈ U).
+ apply G_N; trivial.
+assert (U_0 : ZFnats.zero ∈ U).
+ apply G_inf_nontriv; trivial.
+assert (U_succ : forall n, n ∈ U -> ZFnats.succ n ∈ U).
+ intros.
+ apply G_union2; auto.
+unfold CCLam.
+unfold Lam.Lambda.
+apply G_TI; trivial.
+ do 2 red; intros.
+ unfold Lam.LAMf.
+ rewrite H1; reflexivity.
+
+ intros.
+ unfold Lam.LAMf.
+ auto 20 using G_union2, G_prodcart.
+Qed.
+Hint Resolve G_CCLam.
+
+(** * Encoding of types *)
+
+(** Types are coded by a carrier set X and a realizability relation R
+   assigning a reducibility candidate to each element of the
+   domain.
+   This means that even non-computable functions have "realizers",
+   but no closed ones (it is the set of neutral terms).
+ *)
+Definition mkTY X R := couple X (cc_lam (cc_dec X) (fun x => iSAT (R x))).
+
+Lemma mkTY_ext : forall X Y R R',
+  X == Y ->
+  (forall x x', x ∈ cc_dec X -> x == x' -> eqSAT (R x) (R' x')) ->
+  mkTY X R == mkTY Y R'.
+unfold mkTY; intros.
+apply couple_morph; trivial.
+apply cc_lam_ext; auto.
+ apply cc_dec_morph; trivial.
+red; intros.
+apply iSAT_morph.
+auto.
+Qed.
+
+(* Accessing the set of values of a type.
+   The official membership relation of the model (see inX below) will be
+   x ∈ El T, which reads "x is a value of type T"
+ *)
+Definition Elt T := fst T. (* total elements *)
+Definition El T := union2 (singl empty) (Elt T). (* partial elements *)
+
+Instance Elt_morph : morph1 Elt.
+Proof fst_morph.
+
+Instance El_morph : morph1 El.
+do 2 red; intros; apply union2_morph; auto with *.
+apply fst_morph; trivial.
+Qed.
+
+(* Accessing the realizability relation.
+   inSAT t (Real T x), means that t is a realizer of x in type T. It
+   implicitely requires x ∈ El T. 
+ *)
+Definition Real T x := sSAT (cc_app (snd T) x) .
+
+Instance Real_morph : Proper (eq_set==>eq_set==>eqSAT) Real.
+do 3 red; intros.
+unfold Real.
+apply sSAT_morph.
+rewrite H; rewrite H0; reflexivity.
+Qed.
+
+Lemma Elt_def : forall X R, Elt (mkTY X R) == X.
+unfold El,mkTY; intros.
+apply fst_def.
+Qed.
+
+Lemma El_def : forall X R, El (mkTY X R) == singl empty ∪ X.
+unfold El,Elt,mkTY; intros.
+rewrite fst_def; reflexivity.
+Qed.
+
+Lemma Real_def : forall x X R,
+  (forall x x', x ∈ cc_dec X -> x == x' -> eqSAT (R x) (R x')) ->
+  x ∈ cc_dec X ->
+  eqSAT (Real (mkTY X R) x) (R x).
+intros.
+unfold Real, mkTY.
+rewrite snd_def.
+rewrite cc_beta_eq; auto.
+ apply iSAT_id.
+
+ do 2 red; intros.
+ apply iSAT_morph; auto.
+Qed.
+
+
+Lemma Elt_El x y : x ∈ Elt y -> x ∈ El y.
+intros; apply union2_intro2; trivial.
+Qed.
+Lemma empty_El y : empty ∈ El y.
+apply union2_intro1; apply singl_intro.
+Qed.
+Hint Resolve Elt_El empty_El.
+
+(** * Universes *)
+
+(** Given K a set of set of values, builds a type of types (a sort), such that:
+    - types are neutral term (hence the Real field of the sort is SN)
+    - for each set of values and each realizability relation, there is a type
+      built from this data.
+ *)
+Definition sn_sort K :=
+   mkTY (sup K (fun P =>
+         repl (cc_arr (cc_dec P) (power CCLam)) (fun R T => T == couple P R /\
+                   forall x, x ∈ cc_dec P -> iSAT (sSAT (cc_app R x)) == cc_app R x)))
+     (fun _ => snSAT).
+
+
+Lemma sort_repl_morph P :
+  ZFrepl.repl_rel (cc_arr (cc_dec P) (power CCLam))
+    (fun R T => T == couple P R /\
+           forall x, x ∈ cc_dec P -> iSAT (sSAT (cc_app R x)) == cc_app R x).
+split; intros.
+ revert H2; apply iff_impl.
+ apply and_iff_morphism.
+  rewrite H0; rewrite H1; reflexivity.
+
+  apply fa_morph; intro z.
+  rewrite H0; reflexivity.
+
+ destruct H0; destruct H1.
+ rewrite H0; rewrite H1; reflexivity.
+Qed.
+Lemma sort_repl_morph2 :
+  Proper (eq_set ==> eq_set) (fun P =>
+         repl (cc_arr (cc_dec P) (power CCLam)) (fun R T => T == couple P R /\
+                   forall x, x ∈ cc_dec P -> iSAT (sSAT (cc_app R x)) == cc_app R x)).
+do 2 red; intros.   
+apply ZFrepl.repl_morph_raw.
+ rewrite H; reflexivity.
+
+ do 3 red; intros.
+ apply and_iff_morphism.
+  rewrite H; rewrite H0; rewrite H1; reflexivity.
+
+  apply fa_morph; intro z.
+  rewrite H; rewrite H0; reflexivity.
+Qed.
+Hint Resolve sort_repl_morph sort_repl_morph2.
+
+Lemma sn_sort_ax T K:
+  T ∈ El (sn_sort K) <->
+  T == empty \/
+  exists2 P, P ∈ K & exists2 R,
+    (forall x x', x ∈ cc_dec P -> x==x' -> eqSAT (R x) (R x')) &
+    T == mkTY P R.
+unfold sn_sort; rewrite El_def.
+rewrite union2_ax.
+apply or_iff_morphism.
+ split; intros.
+  apply singl_elim in H; trivial.
+  apply singl_intro_eq; trivial.
+
+ rewrite sup_ax.
+  apply ex2_morph; auto with *.
+  intros P.
+  rewrite repl_ax.
+   split; intros.
+    destruct H as (R,?,(?,?)).
+    exists (fun x => sSAT (cc_app R x)).
+     intros.
+     apply sSAT_morph.
+     apply cc_app_morph; auto with *.
+
+     rewrite H0; apply couple_morph; auto with *.
+     rewrite cc_eta_eq with (1:=H).
+     apply cc_lam_ext; auto with *.
+     red; intros.
+     symmetry.
+     rewrite <- H3; auto.
+
+    destruct H as (R,?,?).
+    assert (ext_fun (cc_dec P) (fun x : set => iSAT (R x))).
+     do 2 red; intros; apply iSAT_morph; auto.
+    exists (cc_lam (cc_dec P) (fun x => iSAT (R x))).
+     apply cc_prod_intro; intros; auto.
+     apply power_intro; intros.
+     apply subset_elim1 in H3; trivial.
+
+     split; intros; trivial.
+     rewrite cc_beta_eq; trivial.
+     rewrite iSAT_id; reflexivity.
+
+   apply sort_repl_morph.
+   apply sort_repl_morph.
+
+  do 2 red; intros; auto.
+Qed.
+
+
+
+Lemma sn_sort_intro K T A :
+  (forall x x', x ∈ cc_dec T -> x == x' -> eqSAT (A x) (A x')) ->
+  T ∈ K -> mkTY T A ∈ El (sn_sort K).
+intros.
+apply sn_sort_ax; right.
+exists T; trivial.
+exists A; auto with *.
+Qed.
+
+Lemma sn_sort_elim_raw K T :
+  T ∈ El (sn_sort K) ->
+  T == empty \/
+  exists U A, T == mkTY U A /\ U ∈ K /\ forall x x', x∈cc_dec U->x==x'->eqSAT(A x)(A x').
+intro.
+apply sn_sort_ax in H.
+destruct H as [?|(P,?,(R,Rext,eqT))]; auto.
+right.
+exists P; exists R; auto.
+Qed.
+
+Lemma sn_sort_elim K T : T ∈ El (sn_sort K) -> T == empty \/ Elt T ∈ K.
+intros.
+apply sn_sort_elim_raw in H; destruct H as [?|(U,(A,(?,(?,?))))]; auto.
+right; rewrite H.
+unfold Elt, mkTY; rewrite fst_def; trivial.
+Qed.
+
+Lemma sort_incl K1 K2 :
+  K1 ⊆ K2 ->
+  El (sn_sort K1) ⊆ El (sn_sort K2).
+red; intros.
+apply sn_sort_elim_raw in H0; destruct H0 as [?|(U,(A,(?,(?,?))))].
+ rewrite H0; auto.
+
+ rewrite H0; apply sn_sort_intro; auto.
+Qed.
+
+Lemma Real_sort_sn T K : T ∈ El (sn_sort K) -> eqSAT (Real (sn_sort K) T) snSAT.
+intros.
+unfold sn_sort.
+apply Real_def.
+ reflexivity.
+
+ unfold sn_sort in H; rewrite El_def in H; trivial.
+Qed.
+
+Lemma sn_sort_in_type K1 K2 :
+  grot_univ K2 ->
+  omega ∈ K2 ->
+  K1 ∈ K2 ->
+  sn_sort K1 ∈ El (sn_sort K2).
+intros.
+apply sn_sort_intro.
+ reflexivity.
+apply G_sup; intros; auto.
+assert (cc_arr (cc_dec x) (power CCLam) ∈ K2).
+ apply G_cc_prod; intros; auto.
+  apply G_union2; auto.
+   apply G_singl; trivial; apply G_inf_nontriv; trivial.
+   apply G_trans with K1; trivial.
+
+  apply G_power; auto.
+apply G_repl; auto.
+intros.
+destruct H5.
+rewrite H5.
+apply G_couple; trivial.
+ apply G_trans with K1; trivial.
+
+ apply G_trans with (2:=H4); trivial.
+Qed.
+
+Lemma El_in_grot K T :
+  grot_univ K -> 
+  empty ∈ K ->
+  T ∈ El (sn_sort K) ->
+  El T ∈ K.
+intros K_grot K_ne T_in_K.
+assert (Kse : singl empty ∈ K).
+ auto using G_singl.
+apply sn_sort_elim in T_in_K; destruct T_in_K.
+ apply G_union2; trivial.
+ rewrite H.
+ apply G_union; trivial.
+ apply G_subset; trivial.
+ apply G_union; trivial.
+
+ apply G_union2; auto.
+Qed.
+
+Definition sn_props := sn_sort props.
+
+Lemma El_in_props P :
+  P ∈ El sn_props ->
+  El P ∈ props.
+intros.
+apply cc_dec_prop.
+apply sn_sort_elim in H; destruct H; trivial.
+rewrite H.
+apply power_intro; intros.
+apply union_elim in H0; destruct H0.
+apply subset_elim1 in H1.
+apply union_elim in H1; destruct H1.
+apply empty_ax in H2; contradiction.
+Qed.
+
+
+(** * Dependent product *)
+
+(** The realizability relation of a dependent product of domain type A
+   and co-domain family of types F for a  function f:
+   it is the intersection of all reducibility candidates {x}A -> {f(x)}F(x)
+   when x ranges A.
+   Note: {x}A -> {f(x)}F(x) is the set of that map any realizer of x (in A) to a
+   realizer of f(x) (in F(x)). So the intersection of these sets when x ranges El(A)
+   is the set of terms that realize f (in forall x:A. F(x)).
+ *)
+Definition piSAT A (F:set->set) (f:set->set) :=
+  interSAT (fun p:{x|x ∈ El A} =>
+    prodSAT (Real A (proj1_sig p)) (Real (F (proj1_sig p)) (f (proj1_sig p)))).
+
+Lemma piSAT_morph : forall A B F F' f f',
+  A == B ->
+  eq_fun (El A) F F' ->
+  eq_fun (El A) f f' -> 
+  eqSAT (piSAT A F f) (piSAT B F' f').
+unfold piSAT; intros.
+apply interSAT_morph_subset; simpl; intros; auto with *.
+ rewrite H; reflexivity.
+
+ apply prodSAT_morph; auto with *.
+  apply Real_morph; auto with *.
+
+  apply Real_morph; auto with *.
+Qed.
+
+
+Definition prod A F :=
+  mkTY (cc_prod (El A) (fun x => El (F x))) (fun f => piSAT A F (cc_app f)).
+
+Lemma Real_prod : forall dom f F,
+    eq_fun (El dom) F F ->
+    f ∈ El (prod dom F) ->
+    eqSAT (Real (prod dom F) f) (piSAT dom F (cc_app f)).
+unfold prod; intros.
+rewrite El_def in H0; rewrite Real_def; trivial.
+ reflexivity.
+
+ do 2 red; intros.
+ apply piSAT_morph; auto with *.
+ red; intros; apply cc_app_morph; trivial.
+Qed.
+
+Definition lam A F := cc_lam (El A) F.
+
+Definition app := cc_app.
+
+Lemma prod_intro : forall dom f F,
+  ext_fun (El dom) f ->
+  ext_fun (El dom) F ->
+  (forall x, x ∈ El dom -> f x ∈ El (F x)) ->
+  lam dom f ∈ El (prod dom F).
+intros.
+unfold lam, prod.
+rewrite El_def.
+apply union2_intro2.
+apply cc_prod_intro; intros; auto.
+do 2 red; intros.
+apply El_morph.
+apply H0;trivial.
+Qed.
+
+Lemma prod_elim : forall dom f x F,
+  eq_fun (El dom) F F ->
+  f ∈ El (prod dom F) ->
+  x ∈ El dom ->
+  cc_app f x ∈ El (F x).
+intros dom f x F _ H H0.
+unfold prod in H; rewrite El_def in H.
+apply union2_elim in H; destruct H.
+ apply singl_elim in H.
+ rewrite H.
+ rewrite cc_app_empty; auto.
+
+ apply cc_prod_elim with (dom:=El dom) (F:=fun x => El(F x)); trivial.
+Qed.
+
+
+(** * Dependent product and universes *)
+
+Lemma predicative_prod : forall K dom F,
+  grot_univ K ->
+  empty ∈ K ->
+  ext_fun (El dom) F ->
+  dom ∈ El (sn_sort K) ->
+  (forall x, x ∈ El dom -> F x ∈ El (sn_sort K)) ->
+  prod dom F ∈ El (sn_sort K).
+intros K dom F K_grot K_ne ext_F dom_ty F_ty.
+apply sn_sort_intro.
+ intros.
+ apply piSAT_morph; auto with *.
+ red; intros.
+ apply cc_app_morph; trivial.
+
+ apply G_cc_prod; trivial.
+  do 2 red; intros.
+  apply El_morph; auto.
+
+  apply El_in_grot; trivial.
+
+  intros.
+  specialize F_ty with (1:=H).
+  apply El_in_grot; trivial.
+Qed.
+
+Lemma impredicative_prod : forall dom F,
+  ext_fun (El dom) F ->
+  (forall x, x ∈ El dom -> F x ∈ El sn_props) ->
+  prod dom F ∈ El sn_props.
+intros.
+apply sn_sort_intro.
+ intros.
+ apply piSAT_morph; auto with *.
+ red; intros.
+ apply cc_app_morph; trivial.
+
+ apply cc_impredicative_prod; intros.
+ specialize H0 with (1:=H1).
+ apply El_in_props; trivial.
+Qed.
